rocq/active/UPGRADE.md
@@ -1,0 +1,21 @@
+Upgrade Guide
+----------------------------
+
+This directory contains some coq proof files written in coq 8.4. Could you upgrade their syntax to be compatible with coq 8.18? Do not touch other directories.
+
+The structure of the project is written in `./AGENT.md`
+
+Here are the rules:
+
+- LibLN and some other libraries are moved to TLC library, when importing them, the TLC prefix will be required.
+  - e.g. `Require Import LibLN.` should be replaced with `Require Import TLC.LibLN.`.
+- `auto*` tactic with no argument should be replaced with `eauto`
+- `auto*` tactic with 1 argument should be replaced with `eauto using`
+- `Omega` library has been superseded by `Lia`, so `Require Import Omega.` should be replaced with `Require Import Lia.`.
+- All Hint defined in the code should be add into `core` hint database.
+- DO NOT delete code, every line in the original proof is necessary.
+- Your code should not be much longer than the old version, this implies a diverging proving process and should be stopped.
+- start your upgrade from `Fsub.v`, then upgrade and compile other coq files individually, starting from the shortest and gradually proceed to longer ones. Do not use make file to compile the whole directory.
+
+
+Coq 8.18 with compatible TLC are already installed, compile often to verify your revision.
